src/frontend/Main.fst
@@ -10,7 +10,7 @@ let test =
   | [_; fn] ->
     let decls = ParserDriver.parse fn in
     let decls = Binding.bind_prog decls in
-    FStar.IO.print_string (String.concat "\n" (List.map Ast.print_decl decls));
+    // FStar.IO.print_string (String.concat "\n" (List.map Ast.print_decl decls));
     let t_decls = List.map Translate.translate_decl decls in
     FStar.IO.print_string (Target.print_decls t_decls)
   | _ ->
